theories/Ordered4/MonadState.v
@@ -1,0 +1,105 @@
+Require Export PredMonad.Ordered4.Monad.
+
+Import OTNotations.
+
+
+(***
+ *** Monads with State Effects
+ ***)
+
+(* State effects = get and put *)
+Class MonadStateOps `(MOps:MonadOps) `(St:OType) : Type :=
+  {
+    getM : M @t@ St ;
+    putM : St -o> M @t@ OTunit
+  }.
+
+Class MonadState `{MonadStateOps} : Prop :=
+  {
+    monad_state_monad :> Monad MOps;
+
+    monad_state_get :
+      forall `{A:OType} (m : M @t@ A),
+        bindM @o@ getM @o@ (mkOTerm _ (fun _ => m)) =o= m ;
+
+    monad_state_get_put :
+      forall `{A:OType} (f : St -o> OTunit -o> M @t@ A),
+        bindM @o@ getM @o@
+              (mkOTerm (St -o> M @t@ A)
+                       (fun s => bindM @o@ (putM @o@ s) @o@ (f @o@ s)))
+        =o= bindM @o@ getM @o@
+                  (mkOTerm (St -o> M @t@ A) (fun s => f @o@ s @o@ tt)) ;
+
+    monad_state_put_get :
+      forall `{A:OType} s (f : OTunit -o> St -o> M @t@ A),
+        bindM @o@ (putM @o@ s) @o@
+              (mkOTerm (OTunit -o> M @t@ A) (fun u => bindM @o@ getM @o@ (f @o@ u)))
+        =o= bindM @o@ (putM @o@ s) @o@
+                  (mkOTerm (OTunit -o> M @t@ A) (fun u => f @o@ u @o@ s)) ;
+
+    monad_state_put_put :
+      forall `{A:OType} s1 s2 (f : OTunit -o> OTunit -o> M @t@ A),
+        bindM @o@ (putM @o@ s1) @o@
+              (mkOTerm (OTunit -o> M @t@ A)
+                       (fun u => bindM @o@ (putM @o@ s2) @o@ (f @o@ u)))
+        =o= bindM @o@ (putM @o@ s2) @o@ (f @o@ tt)
+  }.
+
+
+(***
+ *** The State Monad Transformer
+ ***)
+
+Instance StateT `(St:OType) `(MOps:MonadOps) :
+  OTypeF (fun `(A:OType) => Pfun St (M @t@ (St *o* A)))
+         (fun `(A:OType) => OTarrow_R St (M @t@ (St *o* A))) :=
+  fun `(A:OType) => St -o> M @t@ (St *o* A).
+
+Set Printing All.
+Typeclasses eauto := debug.
+Instance StateT_MonadOps `(St:OType) `(MOps:MonadOps) : MonadOps (StateT St MOps) :=
+  {returnM :=
+     fun `(A:OType) =>
+       mkOTerm (A -o> St -o> M @t@ (St *o* A))
+               (fun x s => returnM @o@ (s, x));
+   bindM :=
+     fun A B m f =>
+       fun s => do s_x <- m s; f (snd s_x) (fst s_x);
+   lrM := fun {A} _ => LR_Op_fun }.
+
+(* The Monad instance for StateT *)
+Global Instance StateT_Monad : Monad (StateT).
+Proof.
+  constructor; intros; unfold StateT, returnM, bindM, lrM, StateT_MonadOps.
+  - auto with typeclass_instances.
+  - prove_lr_proper.
+  - prove_lr_proper.
+  - intros R1 R2 subR; apply LRFun_Proper_subrelation; apply monad_proper_lrM;
+      apply LRPair_Proper_subrelation; try assumption; reflexivity.
+  - prove_lr.
+  - transitivity (fun s => do s_x <- m s; returnM s_x).
+    + split; build_lr_fun; apply monad_proper_bind; prove_lr.
+    + prove_lr; autorewrite with LR; prove_lr.
+  - prove_lr.
+Qed.
+
+Global Instance StateT_MonadStateOps : MonadStateOps S StateT :=
+  { getM := fun s => returnM (s, s)
+  ; putM := fun s _ => returnM (s, tt)
+  }.
+
+Global Instance StateT_MonadState : MonadState S StateT.
+Proof.
+  constructor; intros;
+    unfold StateT, returnM, bindM, lrM, getM, putM,
+    StateT_MonadOps, StateT_MonadStateOps.
+  - auto with typeclass_instances.
+  - prove_lr_proper.
+  - prove_lr_proper.
+  - prove_lr.
+  - prove_lr.
+  - prove_lr.
+  - prove_lr.
+Qed.
+
+End StateT.
